socketio

test/artifact/pneutube/SocketIO.fst
@@ -7,35 +7,51 @@ open Hacl.Constants
 open FileIO.Types
 open PaddedFileIO
 
+module U64 = FStar.UInt64
+module H64 = Hacl.UInt64
+
 assume val current_state: FStar.HyperStack.mem -> socket -> GTot socket_state
 
-assume val tcp_connect: host: uint8_p -> port:u32 -> s:buffer socket -> Stack sresult
-    (requires (fun _ -> True))
-    (ensures  (fun h0 r h1 -> match r with 
-    	      	              | SocketOk -> 
+assume val tcp_connect: host: uint8_p ->
+  port:u32 ->
+  s:buffer socket{length s = 1 /\ disjoint host s} ->
+  Stack sresult
+    (requires (fun h -> live h host /\ live h s))
+    (ensures  (fun h0 r h1 -> modifies_1 s h0 h1 /\ live h1 s /\ live h0 host /\ (match r with
+    	      	              | SocketOk ->
 			      	let sh = get h1 s 0 in
-				current_state h1 sh = Open))
-assume val tcp_listen: port:u32 -> s:buffer socket -> Stack sresult
-    (requires (fun _ -> True))
-    (ensures  (fun h0 r h1 -> match r with 
-    	      	              | SocketOk -> 
-			      	let sh = get h1 s 0 in
-				current_state h1 sh = Open))
-assume val tcp_accept: l:buffer socket -> s:buffer socket -> Stack sresult
-    (requires (fun h0 -> current_state h0 (get h0 l 0) = Open))
-    (ensures  (fun h0 r h1 -> match r with 
-    	      	              | SocketOk -> 
-			      	let sh = get h1 s 0 in
-				current_state h1 sh = Open))
+				current_state h1 sh = Open
+                               | _ -> True)))
 
-assume val tcp_write_all: s:buffer socket -> uint8_p -> len:u64 -> Stack sresult
-    (requires (fun h0 -> current_state h0 (get h0 s 0) = Open))
-    (ensures  (fun _ r h1 -> r = SocketOk ==> current_state h1 (get h1 s 0) = Open))
+assume val tcp_listen: port:u32 -> s:buffer socket{length s = 1} -> Stack sresult
+    (requires (fun h -> live h s))
+    (ensures  (fun h0 r h1 -> live h1 s /\ modifies_1 s h0 h1
+      /\ (match r with | SocketOk -> let sh = get h1 s 0 in current_state h1 sh = Open
+                      | _ -> True)))
 
-assume val tcp_read_all: s:buffer socket -> buffer u8 -> len:u64 -> Stack sresult
-    (requires (fun h0 -> current_state h0 (get h0 s 0) = Open))
-    (ensures  (fun _ r h1 -> r = SocketOk ==> current_state h1 (get h1 s 0) = Open))
+assume val tcp_accept: l:buffer socket{length l = 1} -> s:buffer socket{length s = 1} -> Stack sresult
+    (requires (fun h -> live h s /\ live h l /\ current_state h (get h l 0) = Open))
+    (ensures  (fun h0 r h1 -> live h1 s /\ modifies_1 s h0 h1
+      /\ (match r with | SocketOk -> let sh = get h1 s 0 in current_state h1 sh = Open
+                      | _ -> True)))
 
-assume val tcp_close: s:buffer socket -> Stack sresult
-    (requires (fun h0 -> current_state h0 (get h0 s 0) = Open))
-    (ensures  (fun _ r h1 -> r = SocketOk ==> current_state h1 (get h1 s 0) = Closed))
+assume val tcp_write_all: s:buffer socket{length s = 1} ->
+  b:uint8_p{disjoint s b} ->
+  len:u64{U64.v len <= length b} ->
+  Stack sresult
+    (requires (fun h0 -> live h0 s /\ live h0 b /\ current_state h0 (get h0 s 0) = Open))
+    (ensures  (fun h0 r h1 -> live h1 s /\ live h1 b /\ modifies_1 b h0 h1
+      /\ (r = SocketOk ==> current_state h1 (get h1 s 0) = Open)))
+
+assume val tcp_read_all: s:buffer socket{length s = 1} ->
+  b:buffer u8{disjoint b s} ->
+  len:u64{length b >= U64.v len} ->
+  Stack sresult
+    (requires (fun h0 -> live h0 s /\ live h0 b /\ current_state h0 (get h0 s 0) = Open))
+    (ensures  (fun h0 r h1 -> live h1 s /\ live h1 b /\ modifies_1 b h0 h1
+      /\ (r = SocketOk ==> current_state h1 (get h1 s 0) = Open)))
+
+assume val tcp_close: s:buffer socket{length s = 1} -> Stack sresult
+    (requires (fun h0 -> live h0 s /\ current_state h0 (get h0 s 0) = Open))
+    (ensures  (fun h0 r h1 -> live h1 s /\ h0 == h1
+      /\ (r = SocketOk ==> current_state h1 (get h1 s 0) = Closed)))
